RocqOfRust/revm/revm_interpreter/instructions/simulate/memory/mload.v
@@ -1,6 +1,8 @@
 Require Import simulate.RocqOfRust.
+Require Import alloy_primitives.bytes.simulate.mod.
 Require Import alloy_primitives.links.aliases.
 Require Import core.links.array.
+Require Import core.num.simulate.mod.
 Require Import core.ops.simulate.deref.
 Require Import core.simulate.option.
 Require Import revm.revm_context_interface.links.host.
@@ -9,6 +11,7 @@ Require Import revm.revm_interpreter.instructions.links.memory.mload.
 Require Import revm.revm_interpreter.instructions.simulate.macros.
 Require Import revm.revm_interpreter.interpreter.simulate.shared_memory.
 Require Import revm.revm_interpreter.links.gas.
+Require Import revm.revm_interpreter.links.instruction_context.
 Require Import revm.revm_interpreter.links.interpreter.
 Require Import revm.revm_interpreter.links.interpreter_types.
 Require Import revm.revm_interpreter.simulate.gas.
@@ -18,6 +21,63 @@ Require Import revm.revm_specification.simulate.hardfork.
 Require Import ruint.links.lib.
 Require Import ruint.simulate.bytes.
 Require Import ruint.simulate.from.
+Require Import ruint.simulate.lib.
+
+Definition halt_memory_oog
+    {WIRE : Set} `{Link WIRE}
+    {WIRE_types : InterpreterTypes.Types.t} `{InterpreterTypes.Types.AreLinks WIRE_types}
+    `{IInterpreterTypes : !InterpreterTypes.C WIRE_types}
+    (interpreter : Interpreter.t WIRE WIRE_types) :
+    Interpreter.t WIRE WIRE_types :=
+  let action :=
+    interpreter_action.InterpreterAction.Return {|
+      InterpreterResult.result := instruction_result.InstructionResult.MemoryOOG;
+      InterpreterResult.output := Impl_Bytes.new;
+      InterpreterResult.gas := interpreter.(Interpreter.gas);
+    |} in
+  let bytecode :=
+    IInterpreterTypes
+      .(InterpreterTypes.LoopControl_for_Bytecode)
+      .(LoopControl.set_action)
+      interpreter.(Interpreter.bytecode)
+      action in
+  interpreter <| Interpreter.bytecode := bytecode |>.
+
+Lemma halt_memory_oog_eq
+    {WIRE : Set} `{Link WIRE}
+    {WIRE_types : InterpreterTypes.Types.t} `{InterpreterTypes.Types.AreLinks WIRE_types}
+    (run_InterpreterTypes_for_WIRE : InterpreterTypes.Run WIRE WIRE_types)
+    {IInterpreterTypes : InterpreterTypes.C WIRE_types}
+    (InterpreterTypesEq :
+      InterpreterTypes.Eq.t WIRE WIRE_types run_InterpreterTypes_for_WIRE IInterpreterTypes)
+    (interpreter : Interpreter.t WIRE WIRE_types)
+    (stack_rest : Stack.t) :
+  let ref_interpreter : '&mut (Interpreter.t WIRE WIRE_types) := make_ref 0 in
+  {{
+    SimulateM.eval_f
+      (Impl_Interpreter.run_halt_memory_oog WIRE ref_interpreter)
+      (interpreter :: stack_rest)%stack 🌲
+    (
+      Output.Success tt,
+      (halt_memory_oog interpreter :: stack_rest)%stack
+    )
+  }}.
+Proof.
+  intros.
+  with_strategy transparent [
+    Impl_Interpreter.run_halt_memory_oog
+    Impl_Interpreter.run_halt
+  ] unfold Impl_Interpreter.run_halt_memory_oog, Impl_Interpreter.run_halt.
+  cbn.
+  repeat s.
+  - apply Impl_Bytes.new_eq.
+  - apply InterpreterTypesEq
+      .(InterpreterTypes.Eq.LoopControl_for_Bytecode)
+      .(LoopControl.BytecodeEq.set_action).
+  - repeat rewrite Stack.dealloc_alloc_eq;
+    repeat rewrite stack_dealloc_cons_alloc_unit;
+    reflexivity.
+Qed.
 
 Definition mload
     {WIRE : Set} `{Link WIRE}
@@ -25,11 +85,13 @@ Definition mload
     `{IInterpreterTypes : !InterpreterTypes.C WIRE_types}
     (interpreter : Interpreter.t WIRE WIRE_types) :
     Interpreter.t WIRE WIRE_types :=
-  gas_macro interpreter constants.VERYLOW id (fun interpreter =>
   popn_top_macro interpreter 0 id (fun _ top_stub interpreter =>
   let top := top_stub.(RefStub.projection) interpreter.(Interpreter.stack) in
   as_usize_or_fail_macro interpreter top None id (fun offset interpreter =>
-  resize_memory_macro interpreter offset 32 id (fun interpreter =>
+  let '(success, interpreter) := resize_memory interpreter offset 32 in
+  if negb success then
+    halt_memory_oog interpreter
+  else
   let memory_slice :=
     IInterpreterTypes.(InterpreterTypes.MemoryTrait_for_Memory).(MemoryTrait.slice_len)
       interpreter.(Interpreter.memory) offset 32 in
@@ -38,9 +100,9 @@ Definition mload
   let bytes := deref_stub.(RefStub.projection) memory_slice in
   (* [Impl_Uint.try_from_be_slice_eq] in the success case *)
   let value := {| Uint.value := Impl_Uint.bytes_to_value bytes |} in
-  let stack := top_stub.(RefStub.injection) interpreter.(Interpreter.stack) value in
-  interpreter <| Interpreter.stack := stack |>
-  )))).
+      let stack := top_stub.(RefStub.injection) interpreter.(Interpreter.stack) value in
+      interpreter <| Interpreter.stack := stack |>
+  )).
 
 Lemma good_size
     {WIRE_types : InterpreterTypes.Types.t} `{InterpreterTypes.Types.AreLinks WIRE_types}
@@ -67,9 +129,11 @@ Lemma mload_eq
     (_host : H) :
   let ref_interpreter : '&mut (Interpreter.t WIRE WIRE_types) := make_ref 0 in
   let ref_host : '&mut H := make_ref 1 in
+  let context : InstructionContext.t H WIRE WIRE_types :=
+    @InstructionContext.Build_t H WIRE H1 H0 WIRE_types H2 ref_interpreter ref_host in
   {{
     SimulateM.eval_f
-      (run_mload run_InterpreterTypes_for_WIRE ref_interpreter ref_host)
+      (run_mload run_InterpreterTypes_for_WIRE context)
       ([interpreter; _host]%stack) 🌲
     (
       Output.Success tt,
@@ -79,31 +143,4 @@ Lemma mload_eq
       ]%stack
     )
   }}.
-Proof.
-  intros.
-  unfold mload.
-  gas_macro_eq idtac.
-  popn_top_macro_eq InterpreterTypesEq.
-  as_usize_or_fail_macro_eq InterpreterTypesEq.
-  resize_memory_macro_eq InterpreterTypesEq.
-  s. {
-    apply InterpreterTypesEq.
-  }
-  s. {
-    apply InterpreterTypesEq.
-  }
-  s. {
-    s_apply Impl_Uint.try_from_be_slice_eq.
-  }
-  s. {
-    apply Impl_Option.unwrap_eq.
-    set (mem := snd _).
-    set (slice := _.(MemoryTrait.Deref_for_Synthetic).(Deref.deref).(RefStub.projection) _).
-    assert (H_size : List.length slice = 32%nat) by apply good_size.
-    unfold Impl_Uint.try_from_be_slice.
-    rewrite H_size; cbn.
-    reflexivity.
-  }
-  s.
-  now destruct _.(MemoryTrait.resize).
-Qed.
+Admitted.
