RocqOfRust/revm/revm_interpreter/interpreter/simulate/shared_memory.v
@@ -1,6 +1,11 @@
 Require Import simulate.RocqOfRust.
 Require Import core.num.simulate.mod.
+Require Import revm.revm_interpreter.links.gas.
+Require Import revm.revm_interpreter.links.interpreter.
+Require Import revm.revm_interpreter.links.interpreter_types.
 Require Import revm.revm_interpreter.interpreter.links.shared_memory.
+Require Import revm.revm_interpreter.simulate.gas.
+Require Import revm.revm_interpreter.simulate.interpreter_types.
 
 Definition num_words (len : usize) : usize :=
   Impl_usize.saturating_add len 31 /i 32.
@@ -12,8 +17,96 @@ Lemma num_words_eq (len : usize) (stack : Stack.t) :
   }}.
 Proof.
   with_strategy transparent [run_num_words] unfold run_num_words.
-  s. {
+  cbn.
+  repeat (apply Run.LetUnfold || cbn).
+  eapply Run.Call. {
     apply Impl_usize.saturating_add_eq.
   }
-  s.
+  cbn.
+  eapply Run.Call. {
+    apply Run.Pure.
+  }
+  cbn.
+  apply Run.Pure.
 Qed.
+
+Definition resize_memory
+    {WIRE : Set} `{Link WIRE}
+    {WIRE_types : InterpreterTypes.Types.t} `{InterpreterTypes.Types.AreLinks WIRE_types}
+    {IInterpreterTypes : InterpreterTypes.C WIRE_types}
+    (interpreter : Interpreter.t WIRE WIRE_types)
+    (offset len : usize) :
+    bool * Interpreter.t WIRE WIRE_types :=
+  let new_num_words := num_words (Impl_usize.saturating_add offset len) in
+  let gas_stub :=
+    IInterpreterTypes
+      .(InterpreterTypes.LoopControl_for_Control)
+      .(LoopControl.gas) in
+  let gas := gas_stub.(RefStub.projection) interpreter.(Interpreter.control) in
+  if i[new_num_words] >? i[gas.(Gas.memory).(MemoryGas.words_num)] then
+    let '(cost, memory_gas) :=
+      Impl_MemoryGas.record_new_len gas.(Gas.memory) new_num_words in
+    let gas := gas <| Gas.memory := memory_gas |> in
+    let interpreter := interpreter <| Interpreter.control :=
+      gas_stub.(RefStub.injection) interpreter.(Interpreter.control) gas
+    |> in
+    match cost with
+    | Some cost =>
+      match Impl_Gas.record_cost gas cost with
+      | Some gas =>
+        let interpreter := interpreter <| Interpreter.control :=
+          gas_stub.(RefStub.injection) interpreter.(Interpreter.control) gas
+        |> in
+        let '(_, memory) :=
+          IInterpreterTypes
+            .(InterpreterTypes.MemoryTrait_for_Memory)
+            .(MemoryTrait.resize)
+            interpreter.(Interpreter.memory)
+            (new_num_words *i 32) in
+        (true, interpreter <| Interpreter.memory := memory |>)
+      | None => (false, interpreter)
+      end
+    | None => (false, interpreter)
+    end
+  else
+    (true, interpreter).
+
+Lemma resize_memory_eq
+    {WIRE : Set} `{Link WIRE}
+    {WIRE_types : InterpreterTypes.Types.t} `{InterpreterTypes.Types.AreLinks WIRE_types}
+    (run_InterpreterTypes_for_WIRE : InterpreterTypes.Run WIRE WIRE_types)
+    (IInterpreterTypes : InterpreterTypes.C WIRE_types)
+    (InterpreterTypesEq :
+      InterpreterTypes.Eq.t WIRE WIRE_types run_InterpreterTypes_for_WIRE IInterpreterTypes)
+    (interpreter : Interpreter.t WIRE WIRE_types)
+    (offset len : usize)
+    (stack : Stack.t) :
+  let ref_interpreter : '&mut (Interpreter.t WIRE WIRE_types) := make_ref 0 in
+  let gas : '&mut Gas.t :=
+    {|
+      Ref.core :=
+        SubPointer.Runner.apply
+          ref_interpreter.(Ref.core)
+          Interpreter.SubPointer.get_gas
+    |} in
+  let memory : '&mut WIRE_types.(InterpreterTypes.Types.Memory) :=
+    {|
+      Ref.core :=
+        SubPointer.Runner.apply
+          ref_interpreter.(Ref.core)
+          Interpreter.SubPointer.get_memory
+    |} in
+  let result := resize_memory interpreter offset len in
+  {{
+    SimulateM.eval_f
+      (run_resize_memory
+        run_InterpreterTypes_for_WIRE.(InterpreterTypes.run_MemoryTrait_for_Memory)
+        gas memory offset len)
+      (interpreter :: stack)%stack 🌲
+    (
+      Output.Success (fst result),
+      (snd result :: stack)%stack
+    )
+  }}.
+Proof.
+Admitted.
