RocqOfRust/revm/revm_interpreter/links/interpreter_InterpreterResult.v
@@ -3,7 +3,7 @@ Require Import links.RocqOfRust.
 Require Import alloy_primitives.bytes.links.mod.
 Require Import revm.revm_interpreter.links.instruction_result.
 Require Import revm_interpreter.links.gas.
-
+Require Import revm.revm_interpreter.interpreter.
 (*
 pub struct InterpreterResult {
     pub result: InstructionResult,
@@ -117,3 +117,24 @@ Module InterpreterResult.
   End SubPointer.
 End InterpreterResult.
 Export (hints) InterpreterResult.
+
+(* impl InterpreterResult { *)
+  Module Impl_InterpreterResult.
+  Definition Self : Set :=
+    InterpreterResult.t.
+
+  Instance run_new
+      (result : InstructionResult.t)
+      (output : Bytes.t)
+      (gas : Gas.t) :
+    Run.Trait
+      interpreter.Impl_revm_interpreter_interpreter_InterpreterResult.new
+        [] [] [ φ result; φ output; φ gas ]
+      Self.
+  Proof.
+    constructor.
+    run_symbolic.
+  Defined.
+  Global Opaque run_new.
+End Impl_InterpreterResult.
+Export (hints) Impl_InterpreterResult.
